restructure project files

coq/Parser_sound.v
@@ -1,7 +1,9 @@
 Require Import Arith List.
-Require Import GallStar.Defs. 
+Require Import GallStar.Defs.
+Require Import GallStar.GeneralLemmas.
 Require Import GallStar.Lex.
 Require Import GallStar.Parser.
+Require Import GallStar.ParserLemmas.
 Require Import GallStar.Prediction.
 Require Import GallStar.Tactics.
 Require Import GallStar.Termination.
@@ -20,145 +22,7 @@ Definition bottomFrameSyms (stk : parser_stack) : list symbol :=
   let fr := bottomFrame stk
   in  fr.(loc).(rpre) ++ fr.(loc).(rsuf).
 
-Lemma multistep_unfold :
-  forall g st a,
-    multistep g st a = 
-    match step g st as res return (step g st = res -> parse_result) with
-    | StepAccept sv => fun _  => Accept sv
-    | StepReject s  => fun _  => Reject s
-    | StepK st'     => fun hs =>
-                         multistep g st' (StepK_st_acc g st st' a hs)
-    | StepError s   => fun _  => Error s
-    end eq_refl.
-Proof.
-  intros; destruct a; auto.
-Qed.              
-
-Lemma multistep_cases' :
-  forall (g   : grammar)
-         (st  : parser_state)
-         (a   : Acc lex_nat_triple (Parser.meas g st))
-         (sr  : step_result)
-         (pr  : parse_result)
-         (heq : step g st = sr),
-    match sr as res return (step g st = res -> parse_result) with
-    | StepAccept sv => fun _ => Accept sv
-    | StepReject s => fun _  => Reject s
-    | StepK st' => fun hs => multistep g st' (StepK_st_acc g st st' a hs)
-    | StepError s => fun _ => Error s
-    end heq = pr
-    -> match pr with
-       | Accept f => sr = StepAccept f
-                     \/ exists st' a', sr = StepK st' 
-                                       /\ multistep g st' a' = Accept f
-       | Reject s => sr = StepReject s
-                     \/ exists st' a', sr = StepK st'
-                                       /\ multistep g st' a' = Reject s
-       | Error s  => sr = StepError s
-                     \/ exists st' a', sr = StepK st'
-                                       /\ multistep g st' a' = Error s
-       end.
-Proof.
-  intros g st a sr pr heq.
-  destruct pr; destruct sr; subst;
-    try solve [ intros; tc | intros h; inv h; auto | intros h; right; eauto ].
-Qed.
-
-Lemma multistep_cases :
-  forall (g : grammar)
-         (st : parser_state)
-         (a  : Acc lex_nat_triple (Parser.meas g st))
-         (pr  : parse_result),
-    multistep g st a = pr
-    -> match pr with
-       | Accept f => step g st = StepAccept f
-                     \/ exists st' a', step g st = StepK st' 
-                                       /\ multistep g st' a' = Accept f
-       | Reject s => step g st = StepReject s
-                     \/ exists st' a', step g st = StepK st'
-                                       /\ multistep g st' a' = Reject s
-       | Error s  => step g st = StepError s
-                     \/ exists st' a', step g st = StepK st'
-                                       /\ multistep g st' a' = Error s
-       end.
-Proof.
-  intros g st a pr hm; subst.
-  rewrite multistep_unfold.
-  eapply multistep_cases'; eauto.
-Qed.
-
-Lemma multistep_accept_cases :
-  forall (g : grammar)
-         (st : parser_state)
-         (a  : Acc lex_nat_triple (Parser.meas g st))
-         (f  : forest),
-    multistep g st a = Accept f
-    -> step g st = StepAccept f
-       \/ exists st' a', step g st = StepK st' 
-                         /\ multistep g st' a' = Accept f.
-Proof.
-  intros g st a f hm; subst.
-  destruct (multistep_cases g st a (Accept f)); auto.
-Qed.
-
-Lemma step_StepAccept_facts :
-  forall g av stk ts v,
-    step g (Pst av stk ts) = StepAccept v
-    -> (exists xo rpre v',
-           stk = (Fr (Loc xo rpre []) v', [])
-           /\ v' = v)
-       /\ ts = [].
-Proof.
-  intros g av stk ts v hs.
-  unfold step in hs; dms; tc.
-  inv hs; repeat eexists; eauto.
-Qed.
-
-Inductive stack_wf (g : grammar) : parser_stack -> Prop :=
-| WF_nil :
-    forall pre suf v,
-      stack_wf g (Fr (Loc None pre suf) v, [])
-| WF_cons :
-    forall x xo' pre pre' suf suf' v v' frs,
-      In (x, pre ++ suf) g
-      -> stack_wf g (Fr (Loc xo' pre' (NT x :: suf')) v', frs) 
-      -> stack_wf g (Fr (Loc (Some x) pre suf) v, 
-                     Fr (Loc xo' pre' (NT x :: suf')) v' :: frs).
-
-Hint Constructors stack_wf.
-
-Inductive stack_derivation (g : grammar) : parser_stack -> list token -> Prop :=
-| SD_nil :
-    forall xo pre suf v w,
-      gamma_derivation g pre w v
-      -> stack_derivation g (Fr (Loc xo pre suf) v, []) w
-| SD_cons :
-    forall xo pre suf v fr' frs wpre wsuf,
-      gamma_derivation g pre wsuf v
-      -> stack_derivation g (fr', frs) wpre
-      -> stack_derivation g (Fr (Loc xo pre suf) v, fr' :: frs) (wpre ++ wsuf).
-
-Hint Constructors stack_derivation.
-
 Ltac inv_sd hsd wpre wsuf hgd hsd' := inversion hsd as [? ? ? ? wpre hgd | ? ? ? ? ? ? wpre wsuf hgd hsd']; subst; clear hsd.
-
-(* MAYBE NOT NECESSARY 
-Lemma stack_derivation_accept_impl_gamma_derivation :
-  forall fr stk g wpre av ts v,
-  bottom_frame fr stk
-  -> stack_derivation g stk wpre v
-  -> step g (Pst av stk ts) = StepAccept v
-  -> gamma_derivation g fr.(loc).(rpre) wpre v.
-Proof.
-  intros fr stk g wpre av ts v hb hsdp hf.
-  apply step_StepAccept_facts in hf.
-  destruct hf as [[xo [rpre [v' [heq heq']]]] hnil].
-  subst.
-  inv hb.
-  inv hsdp.
-  simpl; auto.
-Qed.
- *)
 
 Inductive stack_derivation_invar (g : grammar) (stk : parser_stack) (wsuf w : list token) : Prop :=
 | SD_invar :
@@ -185,13 +49,6 @@ Proof.
   constructor; auto.
 Qed.
 
-Lemma app_nil_r' : forall A (xs : list A), xs = xs ++ [].
-Proof.
-  intros; rewrite app_nil_r; auto.
-Qed.
-
-Ltac rew_nilr xs := replace xs with (xs ++ []) by apply app_nil_r'.
-
 Lemma stack_derivation_cases :
   forall g fr frs w,
     stack_derivation g (fr, frs) w
@@ -209,14 +66,6 @@ Proof.
   repeat eexists; repeat split; auto.
 Qed.
 
-Lemma derivation_app_nil_r :
-  forall g ys w v,
-    gamma_derivation g ys w [v] = gamma_derivation g (ys ++ []) (w ++ []) [v].
-Proof.
-  intros g ys w v.
-  assert (happ : w = w ++ []) by (rewrite <- app_nil_r'; auto); rewrite happ; clear happ.
-Abort.
-
 Lemma forest_app_singleton_node : 
   forall g x ys ys' w w' v v',
     In (x, ys') g
@@ -228,13 +77,6 @@ Proof.
   apply gamma_derivation_app; auto.
   assert (happ : w' = w' ++ []) by (rewrite <- app_nil_r'; auto); rewrite happ; clear happ.
   repeat (econstructor; eauto).
-Qed.
-
-Lemma cons_app_singleton :
-  forall A (x : A) (ys : list A),
-    x :: ys = [x] ++ ys.
-Proof.
-  auto.
 Qed.
 
 Lemma terminal_head_gamma_derivation :
@@ -339,59 +181,6 @@ Proof.
   - destruct l; sis; auto.
 Qed.
 
-Lemma in_rhssForNt_production_in_grammar :
-  forall g x ys,
-    In ys (rhssForNt g x)
-    -> In (x, ys) g.
-Proof.
-  intros g x ys hin.
-  induction g as [| (x', ys') g]; sis; tc.
-  destruct (nt_eq_dec x' x); subst; auto.
-  inv hin; auto.
-Qed.
-
-Lemma llPredict_succ_arg_result_in_grammar :
-  forall g x stk ts ys,
-    llPredict g x stk ts = PredSucc ys
-    -> In (x, ys) g.
-Proof.
-  intros g x stk ts ys hp.
-  apply PredSucc_result_in_rhssForNt in hp.
-  apply in_rhssForNt_production_in_grammar; auto.
-Qed.
-
-Lemma llPredict_ambig_arg_result_in_grammar :
-  forall g x stk ts ys,
-    llPredict g x stk ts = PredAmbig ys
-    -> In (x, ys) g.
-Proof.
-  intros g x stk ts ys hp.
-  apply in_rhssForNt_production_in_grammar.
-  eapply PredAmbig_result_in_rhssForNt; eauto.
-Qed.
-
-Lemma step_preserves_stack_wf_invar :
-  forall g av av' stk stk' ts ts',
-    step g (Pst av stk ts) = StepK (Pst av' stk' ts')
-    -> stack_wf g stk 
-    -> stack_wf g stk'.
-Proof.
-  intros g av av' stk stk' ts ts' hs hw.
-  unfold step in hs.
-  repeat (dmeq h); inv hs; tc.
-  - (* return *)
-    inv hw.
-    inv H10; constructor; auto.
-    rewrite <- app_assoc; auto.
-  - inv hw; auto.
-    constructor; auto.
-    rewrite <- app_assoc; auto.
-  - constructor; simpl; auto.
-    eapply llPredict_succ_arg_result_in_grammar; eauto.
-  - constructor; simpl; auto. 
-    eapply llPredict_ambig_arg_result_in_grammar; eauto.
-Qed.    
-
 Lemma multistep_sound :
   forall (g      : grammar)
          (tri    : nat * nat * nat)
@@ -442,5 +231,4 @@ Proof.
   - intros; apply lex_nat_triple_wf.
   - eapply SD_invar with (wpre := []); auto.
 Qed.
-Print Assumptions parser_sound.
   
