coq/GeneralLemmas.v
@@ -1,0 +1,23 @@
+Require Import List.
+Require Import GallStar.Tactics.
+Import ListNotations.
+
+Lemma app_nil_r' : forall A (xs : list A), xs = xs ++ [].
+Proof.
+  intros; rewrite app_nil_r; auto.
+Qed.
+
+Lemma cons_app_singleton :
+  forall A (x : A) (ys : list A),
+    x :: ys = [x] ++ ys.
+Proof.
+  auto.
+Qed.
+
+Lemma in_singleton_eq :
+  forall A (x x' : A), In x' [x] -> x' = x.
+Proof.
+  intros A x x' Hin.
+  destruct Hin as [Hhd | Htl]; auto.
+  inv Htl.
+Qed.
