coq/ParserLemmas.v
@@ -1,0 +1,154 @@
+Require Import List.
+Require Import GallStar.Defs.
+Require Import GallStar.GeneralLemmas.
+Require Import GallStar.Lex.
+Require Import GallStar.Parser.
+Require Import GallStar.Prediction.
+Require Import GallStar.Tactics.
+Import ListNotations.
+
+(* Lemmas for unfolding / inverting calls to step and multistep *)
+
+Lemma multistep_unfold :
+  forall g st a,
+    multistep g st a = 
+    match step g st as res return (step g st = res -> parse_result) with
+    | StepAccept sv => fun _  => Accept sv
+    | StepReject s  => fun _  => Reject s
+    | StepK st'     => fun hs =>
+                         multistep g st' (StepK_st_acc g st st' a hs)
+    | StepError s   => fun _  => Error s
+    end eq_refl.
+Proof.
+  intros; destruct a; auto.
+Qed.              
+
+Lemma multistep_cases' :
+  forall (g   : grammar)
+         (st  : parser_state)
+         (a   : Acc lex_nat_triple (Parser.meas g st))
+         (sr  : step_result)
+         (pr  : parse_result)
+         (heq : step g st = sr),
+    match sr as res return (step g st = res -> parse_result) with
+    | StepAccept sv => fun _ => Accept sv
+    | StepReject s => fun _  => Reject s
+    | StepK st' => fun hs => multistep g st' (StepK_st_acc g st st' a hs)
+    | StepError s => fun _ => Error s
+    end heq = pr
+    -> match pr with
+       | Accept f => sr = StepAccept f
+                     \/ exists st' a', sr = StepK st' 
+                                       /\ multistep g st' a' = Accept f
+       | Reject s => sr = StepReject s
+                     \/ exists st' a', sr = StepK st'
+                                       /\ multistep g st' a' = Reject s
+       | Error s  => sr = StepError s
+                     \/ exists st' a', sr = StepK st'
+                                       /\ multistep g st' a' = Error s
+       end.
+Proof.
+  intros g st a sr pr heq.
+  destruct pr; destruct sr; subst;
+    try solve [ intros; tc | intros h; inv h; auto | intros h; right; eauto ].
+Qed.
+
+Lemma multistep_cases :
+  forall (g : grammar)
+         (st : parser_state)
+         (a  : Acc lex_nat_triple (Parser.meas g st))
+         (pr  : parse_result),
+    multistep g st a = pr
+    -> match pr with
+       | Accept f => step g st = StepAccept f
+                     \/ exists st' a', step g st = StepK st' 
+                                       /\ multistep g st' a' = Accept f
+       | Reject s => step g st = StepReject s
+                     \/ exists st' a', step g st = StepK st'
+                                       /\ multistep g st' a' = Reject s
+       | Error s  => step g st = StepError s
+                     \/ exists st' a', step g st = StepK st'
+                                       /\ multistep g st' a' = Error s
+       end.
+Proof.
+  intros g st a pr hm; subst.
+  rewrite multistep_unfold.
+  eapply multistep_cases'; eauto.
+Qed.
+
+Lemma multistep_accept_cases :
+  forall (g : grammar)
+         (st : parser_state)
+         (a  : Acc lex_nat_triple (Parser.meas g st))
+         (f  : forest),
+    multistep g st a = Accept f
+    -> step g st = StepAccept f
+       \/ exists st' a', step g st = StepK st' 
+                         /\ multistep g st' a' = Accept f.
+Proof.
+  intros g st a f hm; subst.
+  destruct (multistep_cases g st a (Accept f)); auto.
+Qed.
+
+Lemma step_StepAccept_facts :
+  forall g av stk ts v,
+    step g (Pst av stk ts) = StepAccept v
+    -> (exists xo rpre v',
+           stk = (Fr (Loc xo rpre []) v', [])
+           /\ v' = v)
+       /\ ts = [].
+Proof.
+  intros g av stk ts v hs.
+  unfold step in hs; dms; tc.
+  inv hs; repeat eexists; eauto.
+Qed.
+
+(* A well-formedness invariant for the parser stack *)
+
+Inductive stack_wf (g : grammar) : parser_stack -> Prop :=
+| WF_nil :
+    forall pre suf v,
+      stack_wf g (Fr (Loc None pre suf) v, [])
+| WF_cons :
+    forall x xo' pre pre' suf suf' v v' frs,
+      In (x, pre ++ suf) g
+      -> stack_wf g (Fr (Loc xo' pre' (NT x :: suf')) v', frs) 
+      -> stack_wf g (Fr (Loc (Some x) pre suf) v, 
+                     Fr (Loc xo' pre' (NT x :: suf')) v' :: frs).
+
+Hint Constructors stack_wf.
+
+Lemma step_preserves_stack_wf_invar :
+  forall g av av' stk stk' ts ts',
+    step g (Pst av stk ts) = StepK (Pst av' stk' ts')
+    -> stack_wf g stk 
+    -> stack_wf g stk'.
+Proof.
+  intros g av av' stk stk' ts ts' hs hw.
+  unfold step in hs.
+  repeat (dmeq h); inv hs; tc.
+  - (* return *)
+    inv hw.
+    inv H10; constructor; auto.
+    rewrite <- app_assoc; auto.
+  - inv hw; auto.
+    constructor; auto.
+    rewrite <- app_assoc; auto.
+  - constructor; simpl; auto.
+    eapply llPredict_succ_arg_result_in_grammar; eauto.
+  - constructor; simpl; auto. 
+    eapply llPredict_ambig_arg_result_in_grammar; eauto.
+Qed.    
+
+Inductive stack_derivation (g : grammar) : parser_stack -> list token -> Prop :=
+| SD_nil :
+    forall xo pre suf v w,
+      gamma_derivation g pre w v
+      -> stack_derivation g (Fr (Loc xo pre suf) v, []) w
+| SD_cons :
+    forall xo pre suf v fr' frs wpre wsuf,
+      gamma_derivation g pre wsuf v
+      -> stack_derivation g (fr', frs) wpre
+      -> stack_derivation g (Fr (Loc xo pre suf) v, fr' :: frs) (wpre ++ wsuf).
+
+Hint Constructors stack_derivation.
